<?xml version="1.0"?>
<rdf:RDF xmlns="https://w3id.org/ishikawa-diagram-ontology#"
     xml:base="https://w3id.org/ishikawa-diagram-ontology"
     xmlns:dc="http://purl.org/dc/elements/1.1/"
     xmlns:owl="http://www.w3.org/2002/07/owl#"
     xmlns:rdf="http://www.w3.org/1999/02/22-rdf-syntax-ns#"
     xmlns:xml="http://www.w3.org/XML/1998/namespace"
     xmlns:xsd="http://www.w3.org/2001/XMLSchema#"
     xmlns:foaf="http://xmlns.com/foaf/0.1/"
     xmlns:rdfs="http://www.w3.org/2000/01/rdf-schema#"
     xmlns:vann="http://purl.org/vocab/vann/"
     xmlns:terms="http://purl.org/dc/terms/"
     xmlns:schema="http://schema.org/">
    <owl:Ontology rdf:about="https://w3id.org/ishikawa-diagram-ontology">
        <owl:versionIRI rdf:resource="https://w3id.org/ishikawa-diagram-ontology/0.1.0"/>
        <dc:creator rdf:resource="https://orcid.org/0000-0001-7312-3675"/>
        <dc:creator rdf:resource="https://orcid.org/0000-0002-0791-0176"/>
        <dc:creator rdf:resource="https://orcid.org/0000-0003-4280-670X"/>
        <dc:creator rdf:resource="https://orcid.org/0009-0008-5942-3397"/>
        <dc:title>Ishikawa diagram ontology</dc:title>
        <terms:created rdf:datatype="http://www.w3.org/2001/XMLSchema#dateTime">2025-04-24T12:00:00</terms:created>
        <terms:license rdf:resource="https://creativecommons.org/licenses/by/4.0/"/>
        <terms:publisher rdf:resource="https://www.kuleuven.be/kuleuven/"/>
        <vann:preferredNamespacePrefix>ishi</vann:preferredNamespacePrefix>
        <vann:preferredNamespaceUri>https://w3id.org/ishikawa-diagram-ontology</vann:preferredNamespaceUri>
        <schema:citation>Cite this vocabulary as: Fleiner, C., Yang, D., Vandevelde, S., and Vennekens, J. (2025). Ishikawa diagram ontology 0.1.0. https://w3id.org/ishikawa-diagram-ontology/0.1.0</schema:citation>
        <rdfs:comment xml:lang="en">The Ishikawa ontology aims to provide a data and view model to manage data encoded in Ishikawa diagrams which are also known as fishbone or cause and effect diagram (CED).
Ishikawa diagrams result from (iterative) workshops. Thus, the ontology includes the basic modelling of workshops to create Ishikawa diagrams.</rdfs:comment>
        <owl:versionInfo>0.1.0</owl:versionInfo>
    </owl:Ontology>
    


    <!-- 
    ///////////////////////////////////////////////////////////////////////////////////////
    //
    // Annotation properties
    //
    ///////////////////////////////////////////////////////////////////////////////////////
     -->


    


    <!-- http://purl.org/dc/elements/1.1/contributor -->


    <owl:AnnotationProperty rdf:about="http://purl.org/dc/elements/1.1/contributor"/>
    


    <!-- http://purl.org/dc/elements/1.1/creator -->


    <owl:AnnotationProperty rdf:about="http://purl.org/dc/elements/1.1/creator"/>
    


    <!-- http://purl.org/dc/elements/1.1/title -->


    <owl:AnnotationProperty rdf:about="http://purl.org/dc/elements/1.1/title"/>
    


    <!-- http://purl.org/dc/terms/created -->


    <owl:AnnotationProperty rdf:about="http://purl.org/dc/terms/created"/>
    


    <!-- http://purl.org/dc/terms/issued -->


    <owl:AnnotationProperty rdf:about="http://purl.org/dc/terms/issued"/>
    


    <!-- http://purl.org/dc/terms/license -->


    <owl:AnnotationProperty rdf:about="http://purl.org/dc/terms/license"/>
    


    <!-- http://purl.org/dc/terms/publisher -->


    <owl:AnnotationProperty rdf:about="http://purl.org/dc/terms/publisher"/>
    


    <!-- http://purl.org/vocab/vann/preferredNamespacePrefix -->


    <owl:AnnotationProperty rdf:about="http://purl.org/vocab/vann/preferredNamespacePrefix"/>
    


    <!-- http://purl.org/vocab/vann/preferredNamespaceUri -->


    <owl:AnnotationProperty rdf:about="http://purl.org/vocab/vann/preferredNamespaceUri"/>
    


    <!-- http://schema.org/citation -->


    <owl:AnnotationProperty rdf:about="http://schema.org/citation"/>
    


    <!-- http://xmlns.com/foaf/0.1/mbox -->


    <owl:AnnotationProperty rdf:about="http://xmlns.com/foaf/0.1/mbox"/>
    


    <!-- http://xmlns.com/foaf/0.1/name -->


    <owl:AnnotationProperty rdf:about="http://xmlns.com/foaf/0.1/name"/>
    


    <!-- 
    ///////////////////////////////////////////////////////////////////////////////////////
    //
    // Object Properties
    //
    ///////////////////////////////////////////////////////////////////////////////////////
     -->


    


    <!-- http://www.w3.org/ns/ma-ont#format -->


    <owl:ObjectProperty rdf:about="http://www.w3.org/ns/ma-ont#format">
        <rdfs:comment>The MIME type of the resource (e.g., wrapper or bucket media types, container types), ideally including as much information as possible about the resource such as media type parameters, for example, using the &quot;codecs&quot; parameter [RFC 4281].</rdfs:comment>
        <rdfs:label>format</rdfs:label>
    </owl:ObjectProperty>
    


    <!-- http://www.w3.org/ns/ma-ont#locator -->


    <owl:ObjectProperty rdf:about="http://www.w3.org/ns/ma-ont#locator">
        <rdfs:comment>The logical address at which the resource can be accessed (e.g. a URL, or a DVB URI).</rdfs:comment>
        <rdfs:label>locator</rdfs:label>
    </owl:ObjectProperty>
    


    <!-- http://www.w3.org/ns/oa#hasBody -->


    <owl:ObjectProperty rdf:about="http://www.w3.org/ns/oa#hasBody">
        <rdfs:comment>The object of the relationship is a resource that is a body of the Annotation.</rdfs:comment>
        <rdfs:label>hasBody</rdfs:label>
    </owl:ObjectProperty>
    


    <!-- http://www.w3.org/ns/oa#hasPurpose -->


    <owl:ObjectProperty rdf:about="http://www.w3.org/ns/oa#hasPurpose">
        <rdfs:comment>The purpose served by the resource in the Annotation.</rdfs:comment>
        <rdfs:label>hasPurpose</rdfs:label>
    </owl:ObjectProperty>
    


    <!-- http://www.w3.org/ns/oa#hasSelector -->


    <owl:ObjectProperty rdf:about="http://www.w3.org/ns/oa#hasSelector">
        <rdfs:comment>The object of the relationship is a Selector that describes the segment or region of interest within the source resource. Please note that the domain (oa:ResourceSelection) is not used directly in the Web Annotation model.</rdfs:comment>
        <rdfs:label>hasSelector</rdfs:label>
    </owl:ObjectProperty>
    


    <!-- http://www.w3.org/ns/oa#hasSource -->


    <owl:ObjectProperty rdf:about="http://www.w3.org/ns/oa#hasSource">
        <rdfs:comment>The resource that the ResourceSelection, or its subclass SpecificResource, is refined from, or more specific than. Please note that the domain (oa:ResourceSelection) is not used directly in the Web Annotation model.</rdfs:comment>
        <rdfs:label>hasSource</rdfs:label>
    </owl:ObjectProperty>
    


    <!-- http://www.w3.org/ns/oa#hasTarget -->


    <owl:ObjectProperty rdf:about="http://www.w3.org/ns/oa#hasTarget">
        <rdfs:comment>The relationship between an Annotation and its Target.</rdfs:comment>
        <rdfs:label>hasTarget</rdfs:label>
    </owl:ObjectProperty>
    


    <!-- http://www.w3.org/ns/prov#agent -->


    <owl:ObjectProperty rdf:about="http://www.w3.org/ns/prov#agent">
        <rdfs:comment>The prov:agent property references an prov:Agent which influenced a resource. This property applies to an prov:AgentInfluence, which is given by a subproperty of prov:qualifiedInfluence from the influenced prov:Entity, prov:Activity or prov:Agent.</rdfs:comment>
        <rdfs:label>agent</rdfs:label>
    </owl:ObjectProperty>
    


    <!-- http://www.w3.org/ns/prov#contributed -->


    <owl:ObjectProperty rdf:about="http://www.w3.org/ns/prov#contributed">
        <owl:inverseOf rdf:resource="http://www.w3.org/ns/prov#wasAttributedTo"/>
        <rdfs:domain rdf:resource="http://www.w3.org/ns/prov#Agent"/>
        <rdfs:range rdf:resource="http://www.w3.org/ns/prov#Entity"/>
        <rdfs:comment>Attribution is the ascribing of an entity to an agent.</rdfs:comment>
        <rdfs:label>contributed</rdfs:label>
    </owl:ObjectProperty>
    


    <!-- http://www.w3.org/ns/prov#hadDerivation -->


    <owl:ObjectProperty rdf:about="http://www.w3.org/ns/prov#hadDerivation">
        <owl:inverseOf rdf:resource="http://www.w3.org/ns/prov#wasDerivedFrom"/>
        <rdfs:domain rdf:resource="http://www.w3.org/ns/prov#Entity"/>
        <rdfs:range rdf:resource="http://www.w3.org/ns/prov#Entity"/>
        <rdfs:comment>inverse property of wasDerivedFrom</rdfs:comment>
        <rdfs:label>hadDerivation</rdfs:label>
    </owl:ObjectProperty>
    


    <!-- http://www.w3.org/ns/prov#hadRole -->


    <owl:ObjectProperty rdf:about="http://www.w3.org/ns/prov#hadRole">
        <owl:inverseOf rdf:resource="http://www.w3.org/ns/prov#wasRoleIn"/>
        <rdfs:range rdf:resource="http://www.w3.org/ns/prov#Role"/>
        <rdfs:comment>A role is the function of an entity or agent with respect to an activity, in the context of a usage, generation, invalidation, association, start, and end.</rdfs:comment>
        <rdfs:label>hadRole</rdfs:label>
    </owl:ObjectProperty>
    


    <!-- http://www.w3.org/ns/prov#influenced -->


    <owl:ObjectProperty rdf:about="http://www.w3.org/ns/prov#influenced">
        <owl:inverseOf rdf:resource="http://www.w3.org/ns/prov#wasInfluencedBy"/>
        <rdfs:comment>Influence is the capacity of an entity, activity, or agent to have an effect on the character, development, or behavior of another by means of usage, start, end, generation, invalidation, communication, derivation, attribution, association, or delegation.</rdfs:comment>
        <rdfs:label>influenced</rdfs:label>
    </owl:ObjectProperty>
    


    <!-- http://www.w3.org/ns/prov#influencer -->


    <owl:ObjectProperty rdf:about="http://www.w3.org/ns/prov#influencer">
        <rdfs:comment>This property is used as part of the qualified influence pattern. Subclasses of prov:Influence use these subproperties to reference the resource (Entity, Agent, or Activity) whose influence is being qualified.</rdfs:comment>
        <rdfs:label>influencer</rdfs:label>
    </owl:ObjectProperty>
    


    <!-- http://www.w3.org/ns/prov#qualifiedAssociation -->


    <owl:ObjectProperty rdf:about="http://www.w3.org/ns/prov#qualifiedAssociation">
        <owl:inverseOf rdf:resource="http://www.w3.org/ns/prov#qualifiedAssociationOf"/>
        <rdfs:domain rdf:resource="http://www.w3.org/ns/prov#Association"/>
        <rdfs:range rdf:resource="http://www.w3.org/ns/prov#Activity"/>
        <rdfs:comment>An activity association is an assignment of responsibility to an agent for an activity, indicating that the agent had a role in the activity. It further allows for a plan to be specified, which is the plan intended by the agent to achieve some goals in the context of this activity.</rdfs:comment>
        <rdfs:label>qualifiedAssociation</rdfs:label>
    </owl:ObjectProperty>
    


    <!-- http://www.w3.org/ns/prov#qualifiedAssociationOf -->


    <owl:ObjectProperty rdf:about="http://www.w3.org/ns/prov#qualifiedAssociationOf">
        <rdfs:domain rdf:resource="http://www.w3.org/ns/prov#Activity"/>
        <rdfs:range rdf:resource="http://www.w3.org/ns/prov#Association"/>
        <rdfs:label>qualifiedAssociationOf</rdfs:label>
    </owl:ObjectProperty>
    


    <!-- http://www.w3.org/ns/prov#qualifiedAttribution -->


    <owl:ObjectProperty rdf:about="http://www.w3.org/ns/prov#qualifiedAttribution">
        <owl:inverseOf rdf:resource="http://www.w3.org/ns/prov#qualifiedAttributionOf"/>
        <rdfs:domain rdf:resource="http://www.w3.org/ns/prov#Entity"/>
        <rdfs:range rdf:resource="http://www.w3.org/ns/prov#Attribution"/>
        <rdfs:comment>Attribution is the ascribing of an entity to an agent. When an entity e is attributed to agent ag, entity e was generated by some unspecified activity that in turn was associated to agent ag. Thus, this relation is useful when the activity is not known, or irrelevant.</rdfs:comment>
        <rdfs:label>qualifiedAttribution</rdfs:label>
    </owl:ObjectProperty>
    


    <!-- http://www.w3.org/ns/prov#qualifiedAttributionOf -->


    <owl:ObjectProperty rdf:about="http://www.w3.org/ns/prov#qualifiedAttributionOf">
        <rdfs:domain rdf:resource="http://www.w3.org/ns/prov#Attribution"/>
        <rdfs:range rdf:resource="http://www.w3.org/ns/prov#Entity"/>
        <rdfs:label>qualifiedAttributionOf</rdfs:label>
    </owl:ObjectProperty>
    


    <!-- http://www.w3.org/ns/prov#qualifiedInfluence -->


    <owl:ObjectProperty rdf:about="http://www.w3.org/ns/prov#qualifiedInfluence">
        <owl:inverseOf rdf:resource="http://www.w3.org/ns/prov#qualifiedInfluenceOf"/>
        <rdfs:range rdf:resource="http://www.w3.org/ns/prov#Influence"/>
        <rdfs:comment>Influence is the capacity of an entity, activity, or agent to have an effect on the character, development, or behavior of another by means of usage, start, end, generation, invalidation, communication, derivation, attribution, association, or delegation.</rdfs:comment>
        <rdfs:label>qualifiedInfluence</rdfs:label>
    </owl:ObjectProperty>
    


    <!-- http://www.w3.org/ns/prov#qualifiedInfluenceOf -->


    <owl:ObjectProperty rdf:about="http://www.w3.org/ns/prov#qualifiedInfluenceOf">
        <rdfs:domain rdf:resource="http://www.w3.org/ns/prov#Influence"/>
        <rdfs:comment>Influence is the capacity of an entity, activity, or agent to have an effect on the character, development, or behavior of another by means of usage, start, end, generation, invalidation, communication, derivation, attribution, association, or delegation.</rdfs:comment>
        <rdfs:label>qualifiedInfluenceOf</rdfs:label>
    </owl:ObjectProperty>
    


    <!-- http://www.w3.org/ns/prov#wasAssociatedFor -->


    <owl:ObjectProperty rdf:about="http://www.w3.org/ns/prov#wasAssociatedFor">
        <owl:inverseOf rdf:resource="http://www.w3.org/ns/prov#wasAssociatedWith"/>
        <rdfs:domain rdf:resource="http://www.w3.org/ns/prov#Agent"/>
        <rdfs:range rdf:resource="http://www.w3.org/ns/prov#Activity"/>
        <rdfs:comment>An activity association is an assignment of responsibility to an agent for an activity, indicating that the agent had a role in the activity. It further allows for a plan to be specified, which is the plan intended by the agent to achieve some goals in the context of this activity.</rdfs:comment>
        <rdfs:label>wasAssociatedFor</rdfs:label>
    </owl:ObjectProperty>
    


    <!-- http://www.w3.org/ns/prov#wasAssociatedWith -->


    <owl:ObjectProperty rdf:about="http://www.w3.org/ns/prov#wasAssociatedWith">
        <rdfs:domain rdf:resource="http://www.w3.org/ns/prov#Activity"/>
        <rdfs:range rdf:resource="http://www.w3.org/ns/prov#Agent"/>
        <rdfs:comment>An activity association is an assignment of responsibility to an agent for an activity, indicating that the agent had a role in the activity. It further allows for a plan to be specified, which is the plan intended by the agent to achieve some goals in the context of this activity.</rdfs:comment>
        <rdfs:label>wasAssociatedWith</rdfs:label>
    </owl:ObjectProperty>
    


    <!-- http://www.w3.org/ns/prov#wasAttributedTo -->


    <owl:ObjectProperty rdf:about="http://www.w3.org/ns/prov#wasAttributedTo">
        <rdfs:domain rdf:resource="http://www.w3.org/ns/prov#Entity"/>
        <rdfs:range rdf:resource="http://www.w3.org/ns/prov#Agent"/>
        <rdfs:comment>Attribution is the ascribing of an entity to an agent.</rdfs:comment>
        <rdfs:label>wasAttributedTo</rdfs:label>
    </owl:ObjectProperty>
    


    <!-- http://www.w3.org/ns/prov#wasDerivedFrom -->


    <owl:ObjectProperty rdf:about="http://www.w3.org/ns/prov#wasDerivedFrom">
        <rdfs:domain rdf:resource="http://www.w3.org/ns/prov#Entity"/>
        <rdfs:range rdf:resource="http://www.w3.org/ns/prov#Entity"/>
        <rdfs:comment>A derivation is a transformation of an entity into another, an update of an entity resulting in a new one, or the construction of a new entity based on a pre-existing entity.</rdfs:comment>
        <rdfs:label>wasDerivedFrom</rdfs:label>
    </owl:ObjectProperty>
    


    <!-- http://www.w3.org/ns/prov#wasInfluencedBy -->


    <owl:ObjectProperty rdf:about="http://www.w3.org/ns/prov#wasInfluencedBy">
        <rdfs:comment>Influence is the capacity of an entity, activity, or agent to have an effect on the character, development, or behavior of another by means of usage, start, end, generation, invalidation, communication, derivation, attribution, association, or delegation.</rdfs:comment>
        <rdfs:label>wasInfluencedBy</rdfs:label>
    </owl:ObjectProperty>
    


    <!-- http://www.w3.org/ns/prov#wasRoleIn -->


    <owl:ObjectProperty rdf:about="http://www.w3.org/ns/prov#wasRoleIn">
        <rdfs:domain rdf:resource="http://www.w3.org/ns/prov#Role"/>
        <rdfs:comment>A role is the function of an entity or agent with respect to an activity, in the context of a usage, generation, invalidation, association, start, and end.</rdfs:comment>
        <rdfs:label>wasRoleIn</rdfs:label>
    </owl:ObjectProperty>
    


    <!-- https://w3id.org/ishikawa-diagram-ontology#cause -->


    <owl:ObjectProperty rdf:about="https://w3id.org/ishikawa-diagram-ontology#cause">
        <rdfs:domain rdf:resource="https://w3id.org/ishikawa-diagram-ontology#CauseEffect"/>
        <rdfs:range rdf:resource="https://w3id.org/ishikawa-diagram-ontology#Cause"/>
        <rdfs:comment>This property is used to link a Cause to CauseEffect .</rdfs:comment>
        <rdfs:label>cause</rdfs:label>
    </owl:ObjectProperty>
    


    <!-- https://w3id.org/ishikawa-diagram-ontology#causeEffect -->


    <owl:ObjectProperty rdf:about="https://w3id.org/ishikawa-diagram-ontology#causeEffect">
        <owl:inverseOf rdf:resource="https://w3id.org/ishikawa-diagram-ontology#isCauseEffectOf"/>
        <rdfs:domain rdf:resource="https://w3id.org/ishikawa-diagram-ontology#Model"/>
        <rdfs:range rdf:resource="https://w3id.org/ishikawa-diagram-ontology#CauseEffect"/>
        <rdfs:comment>Property links CauseEffects to their Model.</rdfs:comment>
        <rdfs:label>causeEffect</rdfs:label>
    </owl:ObjectProperty>
    


    <!-- https://w3id.org/ishikawa-diagram-ontology#causeEffectType -->


    <owl:ObjectProperty rdf:about="https://w3id.org/ishikawa-diagram-ontology#causeEffectType">
        <rdfs:domain rdf:resource="https://w3id.org/ishikawa-diagram-ontology#CauseEffect"/>
        <rdfs:range rdf:resource="https://w3id.org/ishikawa-diagram-ontology#CauseEffectType"/>
        <rdfs:comment>This property is used to link the CauseEffectType to a CauseEffect</rdfs:comment>
        <rdfs:label>causeEffectType</rdfs:label>
    </owl:ObjectProperty>
    


    <!-- https://w3id.org/ishikawa-diagram-ontology#caused -->


    <owl:ObjectProperty rdf:about="https://w3id.org/ishikawa-diagram-ontology#caused">
        <rdfs:subPropertyOf rdf:resource="http://www.w3.org/ns/prov#influenced"/>
        <owl:inverseOf rdf:resource="https://w3id.org/ishikawa-diagram-ontology#wasCausedBy"/>
        <rdfs:domain rdf:resource="https://w3id.org/ishikawa-diagram-ontology#Cause"/>
        <rdfs:range rdf:resource="https://w3id.org/ishikawa-diagram-ontology#Effect"/>
        <rdfs:comment>This property is used to directly link a Cause to an Effect without further qualification. For qualified cause-effect relationships the CauseEffect class is used.</rdfs:comment>
        <rdfs:label>caused</rdfs:label>
    </owl:ObjectProperty>
    


    <!-- https://w3id.org/ishikawa-diagram-ontology#designPattern -->


    <owl:ObjectProperty rdf:about="https://w3id.org/ishikawa-diagram-ontology#designPattern">
        <rdfs:domain rdf:resource="https://w3id.org/ishikawa-diagram-ontology#Diagram"/>
        <rdfs:range rdf:resource="https://w3id.org/ishikawa-diagram-ontology#DesignPattern"/>
        <rdfs:comment>Property specifies which DesignPattern was used in an Ishikawa diagram.</rdfs:comment>
        <rdfs:label>designPattern</rdfs:label>
    </owl:ObjectProperty>
    


    <!-- https://w3id.org/ishikawa-diagram-ontology#diagram -->


    <owl:ObjectProperty rdf:about="https://w3id.org/ishikawa-diagram-ontology#diagram">
        <owl:inverseOf rdf:resource="https://w3id.org/ishikawa-diagram-ontology#model"/>
        <rdfs:domain rdf:resource="https://w3id.org/ishikawa-diagram-ontology#Model"/>
        <rdfs:range rdf:resource="https://w3id.org/ishikawa-diagram-ontology#Diagram"/>
        <rdfs:comment>This property is used to link the (data) model of an Ishikawa diagram to its visual representation.</rdfs:comment>
        <rdfs:label>diagram</rdfs:label>
    </owl:ObjectProperty>
    


    <!-- https://w3id.org/ishikawa-diagram-ontology#diagramType -->


    <owl:ObjectProperty rdf:about="https://w3id.org/ishikawa-diagram-ontology#diagramType">
        <rdfs:domain rdf:resource="https://w3id.org/ishikawa-diagram-ontology#Diagram"/>
        <rdfs:range rdf:resource="https://w3id.org/ishikawa-diagram-ontology#DiagramType"/>
        <rdfs:comment>This property is used to linke the DiagramType to Diagram.</rdfs:comment>
        <rdfs:label>diagramType</rdfs:label>
    </owl:ObjectProperty>
    


    <!-- https://w3id.org/ishikawa-diagram-ontology#effect -->


    <owl:ObjectProperty rdf:about="https://w3id.org/ishikawa-diagram-ontology#effect">
        <rdfs:domain rdf:resource="https://w3id.org/ishikawa-diagram-ontology#CauseEffect"/>
        <rdfs:range rdf:resource="https://w3id.org/ishikawa-diagram-ontology#Effect"/>
        <rdfs:comment>This property is used to link an Effect to CauseEffect .</rdfs:comment>
        <rdfs:label>effect</rdfs:label>
    </owl:ObjectProperty>
    


    <!-- https://w3id.org/ishikawa-diagram-ontology#evidenceType -->


    <owl:ObjectProperty rdf:about="https://w3id.org/ishikawa-diagram-ontology#evidenceType">
        <rdfs:domain rdf:resource="https://w3id.org/ishikawa-diagram-ontology#Evidence"/>
        <rdfs:range rdf:resource="https://w3id.org/ishikawa-diagram-ontology#EvidenceType"/>
        <rdfs:comment>This property is used to link the EvidenceType to an Evidence</rdfs:comment>
        <rdfs:label>evidenceType</rdfs:label>
    </owl:ObjectProperty>
    


    <!-- https://w3id.org/ishikawa-diagram-ontology#factor -->


    <owl:ObjectProperty rdf:about="https://w3id.org/ishikawa-diagram-ontology#factor">
        <owl:inverseOf rdf:resource="https://w3id.org/ishikawa-diagram-ontology#isFactorOf"/>
        <rdfs:domain rdf:resource="https://w3id.org/ishikawa-diagram-ontology#Model"/>
        <rdfs:range rdf:resource="https://w3id.org/ishikawa-diagram-ontology#Factor"/>
        <rdfs:comment>Property links Factors to their Model.</rdfs:comment>
        <rdfs:label>factor</rdfs:label>
    </owl:ObjectProperty>
    


    <!-- https://w3id.org/ishikawa-diagram-ontology#hadRole -->


    <owl:ObjectProperty rdf:about="https://w3id.org/ishikawa-diagram-ontology#hadRole">
        <rdfs:subPropertyOf rdf:resource="http://www.w3.org/ns/prov#hadRole"/>
        <rdfs:range rdf:resource="https://w3id.org/ishikawa-diagram-ontology#Role"/>
        <rdfs:comment>In the context of the Ishikawa ontology, this property is used to assign roles according to the RASCI model.</rdfs:comment>
        <rdfs:label>hadRole</rdfs:label>
    </owl:ObjectProperty>
    


    <!-- https://w3id.org/ishikawa-diagram-ontology#hasEvidence -->


    <owl:ObjectProperty rdf:about="https://w3id.org/ishikawa-diagram-ontology#hasEvidence">
        <rdfs:domain rdf:resource="https://w3id.org/ishikawa-diagram-ontology#CauseEffect"/>
        <rdfs:range rdf:resource="https://w3id.org/ishikawa-diagram-ontology#Evidence"/>
        <rdfs:comment>This property is used to link a CauseEffect to any Evidence.</rdfs:comment>
        <rdfs:label>hasEvidence</rdfs:label>
    </owl:ObjectProperty>
    


    <!-- https://w3id.org/ishikawa-diagram-ontology#hasNamedRange -->


    <owl:ObjectProperty rdf:about="https://w3id.org/ishikawa-diagram-ontology#hasNamedRange">
        <rdfs:domain rdf:resource="https://w3id.org/ishikawa-diagram-ontology#WeightScale"/>
        <rdfs:range rdf:resource="https://w3id.org/ishikawa-diagram-ontology#WeightRange"/>
        <rdfs:comment>This property is used to link a WeightRange to a WeightScale.</rdfs:comment>
        <rdfs:label>hasNamedRange</rdfs:label>
    </owl:ObjectProperty>
    


    <!-- https://w3id.org/ishikawa-diagram-ontology#hasQualitativeEvidence -->


    <owl:ObjectProperty rdf:about="https://w3id.org/ishikawa-diagram-ontology#hasQualitativeEvidence">
        <rdfs:subPropertyOf rdf:resource="https://w3id.org/ishikawa-diagram-ontology#hasEvidence"/>
        <rdfs:domain rdf:resource="https://w3id.org/ishikawa-diagram-ontology#CauseEffect"/>
        <rdfs:range rdf:resource="https://w3id.org/ishikawa-diagram-ontology#Evidence"/>
        <rdfs:comment>This property is used to link a CauseEffect to any Evidence with the assumption that the evidence is qualitative..</rdfs:comment>
        <rdfs:label>hasQualitativeEvidence</rdfs:label>
    </owl:ObjectProperty>
    


    <!-- https://w3id.org/ishikawa-diagram-ontology#hasQuantitativeEvidence -->


    <owl:ObjectProperty rdf:about="https://w3id.org/ishikawa-diagram-ontology#hasQuantitativeEvidence">
        <rdfs:subPropertyOf rdf:resource="https://w3id.org/ishikawa-diagram-ontology#hasEvidence"/>
        <rdfs:domain rdf:resource="https://w3id.org/ishikawa-diagram-ontology#CauseEffect"/>
        <rdfs:range rdf:resource="https://w3id.org/ishikawa-diagram-ontology#Evidence"/>
        <rdfs:comment>This property is used to link a CauseEffect to any Evidence with the assumption that the evidence is quantitative</rdfs:comment>
        <rdfs:label>hasQuantitativeEvidence</rdfs:label>
    </owl:ObjectProperty>
    


    <!-- https://w3id.org/ishikawa-diagram-ontology#hasWeightRange -->


    <owl:ObjectProperty rdf:about="https://w3id.org/ishikawa-diagram-ontology#hasWeightRange">
        <rdfs:domain rdf:resource="https://w3id.org/ishikawa-diagram-ontology#WeightScale"/>
        <rdfs:range rdf:resource="https://w3id.org/ishikawa-diagram-ontology#WeightRange"/>
        <rdfs:comment>This property is used to link a WeightScale to the WeightRange which defines its total range.</rdfs:comment>
        <rdfs:label>hasWeightRange</rdfs:label>
    </owl:ObjectProperty>
    


    <!-- https://w3id.org/ishikawa-diagram-ontology#isCauseEffectOf -->


    <owl:ObjectProperty rdf:about="https://w3id.org/ishikawa-diagram-ontology#isCauseEffectOf">
        <rdfs:domain rdf:resource="https://w3id.org/ishikawa-diagram-ontology#CauseEffect"/>
        <rdfs:range rdf:resource="https://w3id.org/ishikawa-diagram-ontology#Model"/>
        <rdfs:comment>inverse property to causeEffect</rdfs:comment>
        <rdfs:label>isCauseEffectOf</rdfs:label>
    </owl:ObjectProperty>
    


    <!-- https://w3id.org/ishikawa-diagram-ontology#isFactorOf -->


    <owl:ObjectProperty rdf:about="https://w3id.org/ishikawa-diagram-ontology#isFactorOf">
        <rdfs:domain rdf:resource="https://w3id.org/ishikawa-diagram-ontology#Factor"/>
        <rdfs:range rdf:resource="https://w3id.org/ishikawa-diagram-ontology#Model"/>
        <rdfs:comment>inverse property to factor</rdfs:comment>
        <rdfs:label>isFactorOf</rdfs:label>
    </owl:ObjectProperty>
    


    <!-- https://w3id.org/ishikawa-diagram-ontology#model -->


    <owl:ObjectProperty rdf:about="https://w3id.org/ishikawa-diagram-ontology#model">
        <rdfs:domain rdf:resource="https://w3id.org/ishikawa-diagram-ontology#Diagram"/>
        <rdfs:range rdf:resource="https://w3id.org/ishikawa-diagram-ontology#Model"/>
        <rdfs:comment>This property is used to link the visual representation of an Ishikawa diagram to its data model.</rdfs:comment>
        <rdfs:label>model</rdfs:label>
    </owl:ObjectProperty>
    


    <!-- https://w3id.org/ishikawa-diagram-ontology#qualifiedCauseEffect -->


    <owl:ObjectProperty rdf:about="https://w3id.org/ishikawa-diagram-ontology#qualifiedCauseEffect">
        <rdfs:subPropertyOf rdf:resource="http://www.w3.org/ns/prov#qualifiedInfluence"/>
        <owl:inverseOf rdf:resource="https://w3id.org/ishikawa-diagram-ontology#qualifiedCauseEffectOf"/>
        <rdfs:domain rdf:resource="https://w3id.org/ishikawa-diagram-ontology#Factor"/>
        <rdfs:range rdf:resource="https://w3id.org/ishikawa-diagram-ontology#CauseEffect"/>
        <rdfs:comment>This property is used to link a qualified CauseEffect to a Factor.</rdfs:comment>
        <rdfs:label>qualifiedCauseEffect</rdfs:label>
    </owl:ObjectProperty>
    


    <!-- https://w3id.org/ishikawa-diagram-ontology#qualifiedCauseEffectOf -->


    <owl:ObjectProperty rdf:about="https://w3id.org/ishikawa-diagram-ontology#qualifiedCauseEffectOf">
        <rdfs:subPropertyOf rdf:resource="http://www.w3.org/ns/prov#qualifiedInfluenceOf"/>
        <rdfs:domain rdf:resource="https://w3id.org/ishikawa-diagram-ontology#CauseEffect"/>
        <rdfs:range rdf:resource="https://w3id.org/ishikawa-diagram-ontology#Factor"/>
        <rdfs:comment>This property is used to link a qualified CauseEffect to a Factor.</rdfs:comment>
        <rdfs:label>qualifiedCauseEffectOf</rdfs:label>
    </owl:ObjectProperty>
    


    <!-- https://w3id.org/ishikawa-diagram-ontology#scale -->


    <owl:ObjectProperty rdf:about="https://w3id.org/ishikawa-diagram-ontology#scale">
        <rdfs:domain rdf:resource="https://w3id.org/ishikawa-diagram-ontology#Weight"/>
        <rdfs:range rdf:resource="https://w3id.org/ishikawa-diagram-ontology#WeightScale"/>
        <rdfs:comment>The property is used to link the WeigthScale to a Weight.</rdfs:comment>
        <rdfs:label>scale</rdfs:label>
    </owl:ObjectProperty>
    


    <!-- https://w3id.org/ishikawa-diagram-ontology#usedTechnique -->


    <owl:ObjectProperty rdf:about="https://w3id.org/ishikawa-diagram-ontology#usedTechnique">
        <rdfs:domain rdf:resource="https://w3id.org/ishikawa-diagram-ontology#Workshop"/>
        <rdfs:range rdf:resource="https://w3id.org/ishikawa-diagram-ontology#Technique"/>
        <rdfs:comment>Property to indicate which Technique was used in the Workshop</rdfs:comment>
        <rdfs:label>usedTechnique</rdfs:label>
    </owl:ObjectProperty>
    


    <!-- https://w3id.org/ishikawa-diagram-ontology#wasCausedBy -->


    <owl:ObjectProperty rdf:about="https://w3id.org/ishikawa-diagram-ontology#wasCausedBy">
        <rdfs:subPropertyOf rdf:resource="http://www.w3.org/ns/prov#wasInfluencedBy"/>
        <rdfs:domain rdf:resource="https://w3id.org/ishikawa-diagram-ontology#Effect"/>
        <rdfs:range rdf:resource="https://w3id.org/ishikawa-diagram-ontology#Cause"/>
        <rdfs:comment>This property is used to directly link an Effect to a Cause without further qualification. For qualified cause-effect relationships the CauseEffect class is used.</rdfs:comment>
        <rdfs:label>wasCausedBy</rdfs:label>
    </owl:ObjectProperty>
    


    <!-- https://w3id.org/ishikawa-diagram-ontology#weight -->


    <owl:ObjectProperty rdf:about="https://w3id.org/ishikawa-diagram-ontology#weight">
        <rdfs:domain rdf:resource="https://w3id.org/ishikawa-diagram-ontology#CauseEffect"/>
        <rdfs:range rdf:resource="https://w3id.org/ishikawa-diagram-ontology#Weight"/>
        <rdfs:comment>This property is used to link a Weight to a CauseEffect</rdfs:comment>
        <rdfs:label>weight</rdfs:label>
    </owl:ObjectProperty>
    


    <!-- 
    ///////////////////////////////////////////////////////////////////////////////////////
    //
    // Data properties
    //
    ///////////////////////////////////////////////////////////////////////////////////////
     -->


    


    <!-- https://w3id.org/ishikawa-diagram-ontology#depth -->


    <owl:DatatypeProperty rdf:about="https://w3id.org/ishikawa-diagram-ontology#depth">
        <rdfs:domain rdf:resource="https://w3id.org/ishikawa-diagram-ontology#Diagram"/>
        <rdfs:range rdf:resource="http://www.w3.org/2001/XMLSchema#integer"/>
        <rdfs:comment>This property is used to indicate the maximal depth of the visual representation of an Ishikawa diagram.</rdfs:comment>
        <rdfs:label>depth</rdfs:label>
    </owl:DatatypeProperty>
    


    <!-- https://w3id.org/ishikawa-diagram-ontology#enumerated -->


    <owl:DatatypeProperty rdf:about="https://w3id.org/ishikawa-diagram-ontology#enumerated">
        <rdfs:domain rdf:resource="https://w3id.org/ishikawa-diagram-ontology#Diagram"/>
        <rdfs:range rdf:resource="http://www.w3.org/2001/XMLSchema#boolean"/>
        <rdfs:comment>This property is used to indicate, if factors were enumerated in the visual representation of the Ishikawa diagram.</rdfs:comment>
        <rdfs:label>enumerated</rdfs:label>
    </owl:DatatypeProperty>
    


    <!-- https://w3id.org/ishikawa-diagram-ontology#illustratedEvidence -->


    <owl:DatatypeProperty rdf:about="https://w3id.org/ishikawa-diagram-ontology#illustratedEvidence">
        <rdfs:domain rdf:resource="https://w3id.org/ishikawa-diagram-ontology#Diagram"/>
        <rdfs:range rdf:resource="http://www.w3.org/2001/XMLSchema#boolean"/>
        <rdfs:comment>This property is used to indicate, if the evidence basis was emphasized in the visual representation of the Ishikawa diagram.</rdfs:comment>
        <rdfs:label>illustratedEvidence</rdfs:label>
    </owl:DatatypeProperty>
    


    <!-- https://w3id.org/ishikawa-diagram-ontology#illustratedFactorInfluence -->


    <owl:DatatypeProperty rdf:about="https://w3id.org/ishikawa-diagram-ontology#illustratedFactorInfluence">
        <rdfs:domain rdf:resource="https://w3id.org/ishikawa-diagram-ontology#Diagram"/>
        <rdfs:range rdf:resource="http://www.w3.org/2001/XMLSchema#boolean"/>
        <rdfs:comment>This property is used to indicate, if the factors&apos; influence on the problem were emphasized in the visual representation of the Ishikawa diagram.</rdfs:comment>
        <rdfs:label>illustratedFactorInfluence</rdfs:label>
    </owl:DatatypeProperty>
    


    <!-- https://w3id.org/ishikawa-diagram-ontology#illustratedRoles -->


    <owl:DatatypeProperty rdf:about="https://w3id.org/ishikawa-diagram-ontology#illustratedRoles">
        <rdfs:domain rdf:resource="https://w3id.org/ishikawa-diagram-ontology#Diagram"/>
        <rdfs:range rdf:resource="http://www.w3.org/2001/XMLSchema#boolean"/>
        <rdfs:comment>This property is used to indicate, if responsibilities or roles towards factors were included in the visual representation of the Ishikawa diagram.</rdfs:comment>
        <rdfs:label>illustratedRoles</rdfs:label>
    </owl:DatatypeProperty>
    


    <!-- https://w3id.org/ishikawa-diagram-ontology#illustratedWeight -->


    <owl:DatatypeProperty rdf:about="https://w3id.org/ishikawa-diagram-ontology#illustratedWeight">
        <rdfs:domain rdf:resource="https://w3id.org/ishikawa-diagram-ontology#Diagram"/>
        <rdfs:range rdf:resource="http://www.w3.org/2001/XMLSchema#boolean"/>
        <rdfs:comment>This property is used to indicate, if weight differences were emphasized in the visual representation of the Ishikawa diagram.</rdfs:comment>
        <rdfs:label>illustratedWeight</rdfs:label>
    </owl:DatatypeProperty>
    


    <!-- 
    ///////////////////////////////////////////////////////////////////////////////////////
    //
    // Classes
    //
    ///////////////////////////////////////////////////////////////////////////////////////
     -->


    


    <!-- http://www.w3.org/ns/oa#Annotation -->


    <owl:Class rdf:about="http://www.w3.org/ns/oa#Annotation">
        <rdfs:comment>The class for Web Annotations.</rdfs:comment>
        <rdfs:label>Annotation</rdfs:label>
    </owl:Class>
    


    <!-- http://www.w3.org/ns/oa#FragmentSelector -->


    <owl:Class rdf:about="http://www.w3.org/ns/oa#FragmentSelector">
        <rdfs:comment>The FragmentSelector class is used to record the segment of a representation using the IRI fragment specification defined by the representation&apos;s media type.</rdfs:comment>
        <rdfs:label>FragmentSelector</rdfs:label>
    </owl:Class>
    


    <!-- http://www.w3.org/ns/oa#Motivation -->


    <owl:Class rdf:about="http://www.w3.org/ns/oa#Motivation">
        <rdfs:comment>The Motivation class is used to record the user&apos;s intent or motivation for the creation of the Annotation, or the inclusion of the body or target, that it is associated with.</rdfs:comment>
        <rdfs:label>Motivation</rdfs:label>
    </owl:Class>
    


    <!-- http://www.w3.org/ns/oa#SpecificResource -->


    <owl:Class rdf:about="http://www.w3.org/ns/oa#SpecificResource">
        <rdfs:comment>The SpecificResource refers to the source resource and the constraints that make it more specific.</rdfs:comment>
        <rdfs:label>SpecificResource</rdfs:label>
    </owl:Class>
    


    <!-- http://www.w3.org/ns/oa#TextualBody -->


    <owl:Class rdf:about="http://www.w3.org/ns/oa#TextualBody">
        <rdfs:comment>In many situations, the Body of the Annotation will be in a text format, and created at the same time as the Annotation without a separate IRI. In these cases, the Body&apos;s text can be included as part of the Annotation to avoid having to interact with multiple systems. The Body may also have the features of External Web Resources, including especially the language of the text and the format that it is conveyed in.</rdfs:comment>
        <rdfs:label>TextualBody</rdfs:label>
    </owl:Class>
    


    <!-- http://www.w3.org/ns/prov#Activity -->


    <owl:Class rdf:about="http://www.w3.org/ns/prov#Activity">
        <rdfs:comment>An activity is something that occurs over a period of time and acts upon or with entities; it may include consuming, processing, transforming, modifying, relocating, using, or generating entities.</rdfs:comment>
        <rdfs:label>Activity</rdfs:label>
    </owl:Class>
    


    <!-- http://www.w3.org/ns/prov#Agent -->


    <owl:Class rdf:about="http://www.w3.org/ns/prov#Agent">
        <rdfs:comment>An agent is something that bears some form of responsibility for an activity taking place, for the existence of an entity, or for another agent&apos;s activity.</rdfs:comment>
        <rdfs:label>Agent</rdfs:label>
    </owl:Class>
    


    <!-- http://www.w3.org/ns/prov#Association -->


    <owl:Class rdf:about="http://www.w3.org/ns/prov#Association">
        <rdfs:comment>An activity association is an assignment of responsibility to an agent for an activity, indicating that the agent had a role in the activity. It further allows for a plan to be specified, which is the plan intended by the agent to achieve some goals in the context of this activity.</rdfs:comment>
        <rdfs:label>Association</rdfs:label>
    </owl:Class>
    


    <!-- http://www.w3.org/ns/prov#Attribution -->


    <owl:Class rdf:about="http://www.w3.org/ns/prov#Attribution">
        <rdfs:comment>Attribution is the ascribing of an entity to an agent. When an entity e is attributed to agent ag, entity e was generated by some unspecified activity that in turn was associated to agent ag. Thus, this relation is useful when the activity is not known, or irrelevant.</rdfs:comment>
        <rdfs:label>Attribution</rdfs:label>
    </owl:Class>
    


    <!-- http://www.w3.org/ns/prov#Bundle -->


    <owl:Class rdf:about="http://www.w3.org/ns/prov#Bundle">
        <rdfs:comment>A bundle is a named set of provenance descriptions, and is itself an Entity, so allowing provenance of provenance to be expressed.</rdfs:comment>
        <rdfs:label>Bundle</rdfs:label>
    </owl:Class>
    


    <!-- http://www.w3.org/ns/prov#Entity -->


    <owl:Class rdf:about="http://www.w3.org/ns/prov#Entity">
        <rdfs:comment>An entity is a physical, digital, conceptual, or other kind of thing with some fixed aspects; entities may be real or imaginary.</rdfs:comment>
        <rdfs:label>Entity</rdfs:label>
    </owl:Class>
    


    <!-- http://www.w3.org/ns/prov#Influence -->


    <owl:Class rdf:about="http://www.w3.org/ns/prov#Influence">
        <rdfs:comment>Influence is the capacity of an entity, activity, or agent to have an effect on the character, development, or behavior of another by means of usage, start, end, generation, invalidation, communication, derivation, attribution, association, or delegation.</rdfs:comment>
        <rdfs:label>Influence</rdfs:label>
    </owl:Class>
    


    <!-- http://www.w3.org/ns/prov#Role -->


    <owl:Class rdf:about="http://www.w3.org/ns/prov#Role">
        <rdfs:comment>A role is the function of an entity or agent with respect to an activity, in the context of a usage, generation, invalidation, association, start, and end.</rdfs:comment>
        <rdfs:label>Role</rdfs:label>
    </owl:Class>
    


    <!-- https://w3id.org/ishikawa-diagram-ontology#Cause -->


    <owl:Class rdf:about="https://w3id.org/ishikawa-diagram-ontology#Cause">
        <rdfs:subClassOf rdf:resource="https://w3id.org/ishikawa-diagram-ontology#Factor"/>
        <rdfs:comment>A cause is a factor where its characteristics has direct influence on the characteristics of another factor.</rdfs:comment>
        <rdfs:label>Cause</rdfs:label>
    </owl:Class>
    


    <!-- https://w3id.org/ishikawa-diagram-ontology#CauseEffect -->


    <owl:Class rdf:about="https://w3id.org/ishikawa-diagram-ontology#CauseEffect">
        <rdfs:subClassOf rdf:resource="http://www.w3.org/ns/prov#Influence"/>
        <rdfs:comment>CauseEffect is the capacity of a factor to have an effect on the character of another. The class is used to record qualified cause-effect relationships.</rdfs:comment>
        <rdfs:label>CauseEffect</rdfs:label>
    </owl:Class>
    


    <!-- https://w3id.org/ishikawa-diagram-ontology#CauseEffectType -->


    <owl:Class rdf:about="https://w3id.org/ishikawa-diagram-ontology#CauseEffectType">
        <rdfs:comment>The class is used to record the type of cause-effect relationship that exists between at least one cause and at least one effect.</rdfs:comment>
        <rdfs:label>CauseEffectType</rdfs:label>
    </owl:Class>
    


    <!-- https://w3id.org/ishikawa-diagram-ontology#CertaintyScale -->


    <owl:Class rdf:about="https://w3id.org/ishikawa-diagram-ontology#CertaintyScale">
        <rdfs:subClassOf rdf:resource="https://w3id.org/ishikawa-diagram-ontology#WeightScale"/>
        <rdfs:comment>A WeightScale where the numerical weight refers to the certainty.</rdfs:comment>
        <rdfs:label>CertaintyScale</rdfs:label>
    </owl:Class>
    


    <!-- https://w3id.org/ishikawa-diagram-ontology#DesignPattern -->


    <owl:Class rdf:about="https://w3id.org/ishikawa-diagram-ontology#DesignPattern">
        <rdfs:comment>The class is used to record the design pattern which was applied in the course of the Ishikawa diagram creation. Instances of the class refer to best practices.</rdfs:comment>
        <rdfs:label>DesignPattern</rdfs:label>
    </owl:Class>
    


    <!-- https://w3id.org/ishikawa-diagram-ontology#Diagram -->


    <owl:Class rdf:about="https://w3id.org/ishikawa-diagram-ontology#Diagram">
        <rdfs:subClassOf rdf:resource="http://www.w3.org/ns/prov#Entity"/>
        <rdfs:comment>A visual representation of an Ishikawa diagram model or of a portion of it.</rdfs:comment>
        <rdfs:label>Diagram</rdfs:label>
    </owl:Class>
    


    <!-- https://w3id.org/ishikawa-diagram-ontology#DiagramType -->


    <owl:Class rdf:about="https://w3id.org/ishikawa-diagram-ontology#DiagramType">
        <rdfs:comment>The class is used to record the type of the Ishikawa diagram</rdfs:comment>
        <rdfs:label>DiagramType</rdfs:label>
    </owl:Class>
    


    <!-- https://w3id.org/ishikawa-diagram-ontology#Effect -->


    <owl:Class rdf:about="https://w3id.org/ishikawa-diagram-ontology#Effect">
        <rdfs:subClassOf rdf:resource="https://w3id.org/ishikawa-diagram-ontology#Factor"/>
        <rdfs:comment>An effect is a factor where its characteristics are directly influenced by the characteristics of another factor.</rdfs:comment>
        <rdfs:label>Effect</rdfs:label>
    </owl:Class>
    


    <!-- https://w3id.org/ishikawa-diagram-ontology#Evidence -->


    <owl:Class rdf:about="https://w3id.org/ishikawa-diagram-ontology#Evidence">
        <rdfs:comment>Evidence refers to all resources that (partially) validate a cause-effeect relationship.</rdfs:comment>
        <rdfs:label>Evidence</rdfs:label>
    </owl:Class>
    


    <!-- https://w3id.org/ishikawa-diagram-ontology#EvidenceType -->


    <owl:Class rdf:about="https://w3id.org/ishikawa-diagram-ontology#EvidenceType">
        <rdfs:comment>The class is used to specify Evidence resources.</rdfs:comment>
        <rdfs:label>EvidenceType</rdfs:label>
    </owl:Class>
    


    <!-- https://w3id.org/ishikawa-diagram-ontology#Factor -->


    <owl:Class rdf:about="https://w3id.org/ishikawa-diagram-ontology#Factor">
        <rdfs:subClassOf>
            <owl:Class>
                <owl:unionOf rdf:parseType="Collection">
                    <rdf:Description rdf:about="http://www.w3.org/ns/prov#Activity"/>
                    <rdf:Description rdf:about="http://www.w3.org/ns/prov#Entity"/>
                </owl:unionOf>
            </owl:Class>
        </rdfs:subClassOf>
        <rdfs:comment>A factor is any activity or entity with identified cause-effect relationships in the context of root-cause analysis</rdfs:comment>
        <rdfs:label>Factor</rdfs:label>
    </owl:Class>
    


    <!-- https://w3id.org/ishikawa-diagram-ontology#ImpactScale -->


    <owl:Class rdf:about="https://w3id.org/ishikawa-diagram-ontology#ImpactScale">
        <rdfs:subClassOf rdf:resource="https://w3id.org/ishikawa-diagram-ontology#WeightScale"/>
        <rdfs:comment>A WeightScale where the numerical weight refers to an imact value. Impact describes the estimated and quantified effect an occurence of a cause-effect relationship might have.</rdfs:comment>
        <rdfs:label>ImpactScale</rdfs:label>
    </owl:Class>
    


    <!-- https://w3id.org/ishikawa-diagram-ontology#MajorCause -->


    <owl:Class rdf:about="https://w3id.org/ishikawa-diagram-ontology#MajorCause">
        <rdfs:subClassOf rdf:resource="https://w3id.org/ishikawa-diagram-ontology#Cause"/>
        <rdfs:comment>A major cause has a direct cause-effect relationship with the root cause in the context of an Ishikawa diagram. When design patterns are used, major causes are abstract causes which are commonly referred to as categories.</rdfs:comment>
        <rdfs:label>MajorCause</rdfs:label>
    </owl:Class>
    


    <!-- https://w3id.org/ishikawa-diagram-ontology#Model -->


    <owl:Class rdf:about="https://w3id.org/ishikawa-diagram-ontology#Model">
        <rdfs:subClassOf rdf:resource="http://www.w3.org/ns/prov#Bundle"/>
        <rdfs:comment>The Model class is used to record factors and their cause-effect relationships. It can be seen as the data model of an Ishikawa diagram.</rdfs:comment>
        <rdfs:label>Model</rdfs:label>
    </owl:Class>
    


    <!-- https://w3id.org/ishikawa-diagram-ontology#ProbabilityScale -->


    <owl:Class rdf:about="https://w3id.org/ishikawa-diagram-ontology#ProbabilityScale">
        <rdfs:subClassOf rdf:resource="https://w3id.org/ishikawa-diagram-ontology#WeightScale"/>
        <rdfs:comment>A WeightScale where the numerical weight refers to a probability value. Probability describes the likelihood of occurence of a cause-effect relationship.</rdfs:comment>
        <rdfs:label>ProbabilityScale</rdfs:label>
    </owl:Class>
    


    <!-- https://w3id.org/ishikawa-diagram-ontology#Problem -->


    <owl:Class rdf:about="https://w3id.org/ishikawa-diagram-ontology#Problem">
        <rdfs:subClassOf rdf:resource="https://w3id.org/ishikawa-diagram-ontology#Effect"/>
        <rdfs:comment>A problem is a factor which does not influence any known factor in the context of an Ishikawa diagram.</rdfs:comment>
        <rdfs:label>Problem</rdfs:label>
    </owl:Class>
    


    <!-- https://w3id.org/ishikawa-diagram-ontology#RelevanceScale -->


    <owl:Class rdf:about="https://w3id.org/ishikawa-diagram-ontology#RelevanceScale">
        <rdfs:subClassOf rdf:resource="https://w3id.org/ishikawa-diagram-ontology#WeightScale"/>
        <rdfs:comment>A WeightScale where the numerical weight refers to a relevance value. Relevance describes the importance a cause-effect relationship has in the context of a root-cause analysis.</rdfs:comment>
        <rdfs:label>RelevanceScale</rdfs:label>
    </owl:Class>
    


    <!-- https://w3id.org/ishikawa-diagram-ontology#RiskScale -->


    <owl:Class rdf:about="https://w3id.org/ishikawa-diagram-ontology#RiskScale">
        <rdfs:subClassOf rdf:resource="https://w3id.org/ishikawa-diagram-ontology#WeightScale"/>
        <rdfs:comment>A WeightScale where the numerical weight refers to a risk value. Risk describes the estimated potential damage the occurence of a cause-effect relationship might have. Risk is often calculated as the product of probability and impact.</rdfs:comment>
        <rdfs:label>RiskScale</rdfs:label>
    </owl:Class>
    


    <!-- https://w3id.org/ishikawa-diagram-ontology#Role -->


    <owl:Class rdf:about="https://w3id.org/ishikawa-diagram-ontology#Role">
        <rdfs:subClassOf rdf:resource="http://www.w3.org/ns/prov#Role"/>
        <rdfs:comment>A role is the function of an agent with respect to a factor. The ontology incorporates role instances adhering to the RASCI model.</rdfs:comment>
        <rdfs:label>Role</rdfs:label>
    </owl:Class>
    


    <!-- https://w3id.org/ishikawa-diagram-ontology#RootCause -->


    <owl:Class rdf:about="https://w3id.org/ishikawa-diagram-ontology#RootCause">
        <rdfs:subClassOf rdf:resource="https://w3id.org/ishikawa-diagram-ontology#Cause"/>
        <rdfs:comment>A root cause is a factor which is not influenced by any known factor in the context of an Ishikawa diagram.</rdfs:comment>
        <rdfs:label>RootCause</rdfs:label>
    </owl:Class>
    


    <!-- https://w3id.org/ishikawa-diagram-ontology#Technique -->


    <owl:Class rdf:about="https://w3id.org/ishikawa-diagram-ontology#Technique">
        <rdfs:subClassOf rdf:resource="https://w3id.org/pko#Procedure"/>
        <rdfs:comment>An established activity with the goal of peperapring or creating an Ishikawa diagram</rdfs:comment>
        <rdfs:label>Technique</rdfs:label>
    </owl:Class>
    


    <!-- https://w3id.org/ishikawa-diagram-ontology#Weight -->


    <owl:Class rdf:about="https://w3id.org/ishikawa-diagram-ontology#Weight">
        <rdfs:comment>The weight class is used to assign values to a cause-effect relationship for priorization. The intended meaning of the weight depends on the referenced WeightScale</rdfs:comment>
        <rdfs:label>Weight</rdfs:label>
    </owl:Class>
    


    <!-- https://w3id.org/ishikawa-diagram-ontology#WeightRange -->


    <owl:Class rdf:about="https://w3id.org/ishikawa-diagram-ontology#WeightRange">
        <rdfs:comment>The WeightRange class is used to specify and name subranges.</rdfs:comment>
        <rdfs:label>WeightRange</rdfs:label>
    </owl:Class>
    


    <!-- https://w3id.org/ishikawa-diagram-ontology#WeightScale -->


    <owl:Class rdf:about="https://w3id.org/ishikawa-diagram-ontology#WeightScale">
        <rdfs:comment>A class that specifies the min and max range of values for the weight of a cause-effect relationship.</rdfs:comment>
        <rdfs:label>WeightScale</rdfs:label>
    </owl:Class>
    


    <!-- https://w3id.org/ishikawa-diagram-ontology#Workshop -->


    <owl:Class rdf:about="https://w3id.org/ishikawa-diagram-ontology#Workshop">
        <rdfs:subClassOf rdf:resource="https://w3id.org/pko#ProcedureExecution"/>
        <rdfs:comment>A structured or guided activity to create an Ishikawa diagram</rdfs:comment>
        <rdfs:label>Workshop</rdfs:label>
    </owl:Class>
    


    <!-- https://w3id.org/pko#Procedure -->


    <owl:Class rdf:about="https://w3id.org/pko#Procedure">
        <rdfs:comment>A Procedure represents a sequence of actions to be executed in order to achieve a desired outcome.</rdfs:comment>
        <rdfs:label>Procedure</rdfs:label>
    </owl:Class>
    


    <!-- https://w3id.org/pko#ProcedureExecution -->


    <owl:Class rdf:about="https://w3id.org/pko#ProcedureExecution">
        <rdfs:comment>A Procedure Execution is an Activity representing the execution of a certain Procedure, performed by one or more Agents, during a time interval.</rdfs:comment>
        <rdfs:label>ProcedureExecution</rdfs:label>
    </owl:Class>
    


    <!-- 
    ///////////////////////////////////////////////////////////////////////////////////////
    //
    // Individuals
    //
    ///////////////////////////////////////////////////////////////////////////////////////
     -->


    


    <!-- http://www.w3.org/ns/oa#highlighting -->


    <owl:NamedIndividual rdf:about="http://www.w3.org/ns/oa#highlighting">
        <rdf:type rdf:resource="http://www.w3.org/ns/oa#Motivation"/>
        <rdfs:comment>The motivation for when the user intends to highlight the Target resource or segment of it.</rdfs:comment>
    </owl:NamedIndividual>
    


    <!-- https://orcid.org/0000-0001-7312-3675 -->


    <owl:NamedIndividual rdf:about="https://orcid.org/0000-0001-7312-3675">
        <rdfs:label>Simon Vandevelde</rdfs:label>
        <foaf:name>Simon Vandevelde</foaf:name>
    </owl:NamedIndividual>
    


    <!-- https://orcid.org/0000-0002-0791-0176 -->


    <owl:NamedIndividual rdf:about="https://orcid.org/0000-0002-0791-0176">
        <rdfs:label>Joost Vennekens</rdfs:label>
        <foaf:name>Joost Vennekens</foaf:name>
    </owl:NamedIndividual>
    


    <!-- https://orcid.org/0000-0003-4280-670X -->


    <owl:NamedIndividual rdf:about="https://orcid.org/0000-0003-4280-670X">
        <rdfs:label>Christian Fleiner</rdfs:label>
        <foaf:name>Christian Fleiner</foaf:name>
    </owl:NamedIndividual>
    


    <!-- https://orcid.org/0009-0008-5942-3397 -->


    <owl:NamedIndividual rdf:about="https://orcid.org/0009-0008-5942-3397">
        <rdfs:label>Duo Yang</rdfs:label>
        <foaf:name>Duo Yang</foaf:name>
    </owl:NamedIndividual>
    


    <!-- https://w3id.org/ishikawa-diagram-ontology#Accountable -->


    <owl:NamedIndividual rdf:about="https://w3id.org/ishikawa-diagram-ontology#Accountable">
        <rdf:type rdf:resource="https://w3id.org/ishikawa-diagram-ontology#Role"/>
    </owl:NamedIndividual>
    


    <!-- https://w3id.org/ishikawa-diagram-ontology#Consulted -->


    <owl:NamedIndividual rdf:about="https://w3id.org/ishikawa-diagram-ontology#Consulted">
        <rdf:type rdf:resource="https://w3id.org/ishikawa-diagram-ontology#Role"/>
    </owl:NamedIndividual>
    


    <!-- https://w3id.org/ishikawa-diagram-ontology#DoE -->


    <owl:NamedIndividual rdf:about="https://w3id.org/ishikawa-diagram-ontology#DoE">
        <rdf:type rdf:resource="https://w3id.org/ishikawa-diagram-ontology#DesignPattern"/>
        <rdfs:comment xml:lang="en">The categories are &quot;uncontrollable factors&quot;, &quot;controllable factors&quot;, &quot;blockable nuisance factors&quot;, and &quot;held-constant factors&quot;</rdfs:comment>
        <rdfs:label xml:lang="en">Design of experiments</rdfs:label>
    </owl:NamedIndividual>
    


    <!-- https://w3id.org/ishikawa-diagram-ontology#Informed -->


    <owl:NamedIndividual rdf:about="https://w3id.org/ishikawa-diagram-ontology#Informed">
        <rdf:type rdf:resource="https://w3id.org/ishikawa-diagram-ontology#Role"/>
    </owl:NamedIndividual>
    


    <!-- https://w3id.org/ishikawa-diagram-ontology#Responsible -->


    <owl:NamedIndividual rdf:about="https://w3id.org/ishikawa-diagram-ontology#Responsible">
        <rdf:type rdf:resource="https://w3id.org/ishikawa-diagram-ontology#Role"/>
    </owl:NamedIndividual>
    


    <!-- https://w3id.org/ishikawa-diagram-ontology#STEPC -->


    <owl:NamedIndividual rdf:about="https://w3id.org/ishikawa-diagram-ontology#STEPC">
        <rdf:type rdf:resource="https://w3id.org/ishikawa-diagram-ontology#DesignPattern"/>
        <rdfs:comment xml:lang="en">The categories are &quot;site&quot;, &quot;task&quot;, &quot;equipment&quot;, &quot;people&quot;, and &quot;control&quot;</rdfs:comment>
        <rdfs:label xml:lang="en">STEPC method</rdfs:label>
    </owl:NamedIndividual>
    


    <!-- https://w3id.org/ishikawa-diagram-ontology#Supporting -->


    <owl:NamedIndividual rdf:about="https://w3id.org/ishikawa-diagram-ontology#Supporting">
        <rdf:type rdf:resource="https://w3id.org/ishikawa-diagram-ontology#Role"/>
    </owl:NamedIndividual>
    


    <!-- https://w3id.org/ishikawa-diagram-ontology#aggravating -->


    <owl:NamedIndividual rdf:about="https://w3id.org/ishikawa-diagram-ontology#aggravating">
        <rdf:type rdf:resource="https://w3id.org/ishikawa-diagram-ontology#CauseEffectType"/>
    </owl:NamedIndividual>
    


    <!-- https://w3id.org/ishikawa-diagram-ontology#causeEnumerationDiagram -->


    <owl:NamedIndividual rdf:about="https://w3id.org/ishikawa-diagram-ontology#causeEnumerationDiagram">
        <rdf:type rdf:resource="https://w3id.org/ishikawa-diagram-ontology#DiagramType"/>
    </owl:NamedIndividual>
    


    <!-- https://w3id.org/ishikawa-diagram-ontology#dispersionAnalysisDiagram -->


    <owl:NamedIndividual rdf:about="https://w3id.org/ishikawa-diagram-ontology#dispersionAnalysisDiagram">
        <rdf:type rdf:resource="https://w3id.org/ishikawa-diagram-ontology#DiagramType"/>
    </owl:NamedIndividual>
    


    <!-- https://w3id.org/ishikawa-diagram-ontology#neutralizing -->


    <owl:NamedIndividual rdf:about="https://w3id.org/ishikawa-diagram-ontology#neutralizing">
        <rdf:type rdf:resource="https://w3id.org/ishikawa-diagram-ontology#CauseEffectType"/>
    </owl:NamedIndividual>
    


    <!-- https://w3id.org/ishikawa-diagram-ontology#noEvidence -->


    <owl:NamedIndividual rdf:about="https://w3id.org/ishikawa-diagram-ontology#noEvidence">
        <rdf:type rdf:resource="https://w3id.org/ishikawa-diagram-ontology#EvidenceType"/>
    </owl:NamedIndividual>
    


    <!-- https://w3id.org/ishikawa-diagram-ontology#productProcessClassificationDiagram -->


    <owl:NamedIndividual rdf:about="https://w3id.org/ishikawa-diagram-ontology#productProcessClassificationDiagram">
        <rdf:type rdf:resource="https://w3id.org/ishikawa-diagram-ontology#DiagramType"/>
    </owl:NamedIndividual>
    


    <!-- https://w3id.org/ishikawa-diagram-ontology#qualitativeEvidence -->


    <owl:NamedIndividual rdf:about="https://w3id.org/ishikawa-diagram-ontology#qualitativeEvidence">
        <rdf:type rdf:resource="https://w3id.org/ishikawa-diagram-ontology#EvidenceType"/>
    </owl:NamedIndividual>
    


    <!-- https://w3id.org/ishikawa-diagram-ontology#quantitativeEvidence -->


    <owl:NamedIndividual rdf:about="https://w3id.org/ishikawa-diagram-ontology#quantitativeEvidence">
        <rdf:type rdf:resource="https://w3id.org/ishikawa-diagram-ontology#EvidenceType"/>
    </owl:NamedIndividual>
    


    <!-- https://w3id.org/ishikawa-diagram-ontology#undecided -->


    <owl:NamedIndividual rdf:about="https://w3id.org/ishikawa-diagram-ontology#undecided">
        <rdf:type rdf:resource="https://w3id.org/ishikawa-diagram-ontology#CauseEffectType"/>
    </owl:NamedIndividual>
    


    <!-- https://w3id.org/ishikawa-diagram-ontology#4S -->


    <owl:NamedIndividual rdf:about="https://w3id.org/ishikawa-diagram-ontology#4S">
        <rdf:type rdf:resource="https://w3id.org/ishikawa-diagram-ontology#DesignPattern"/>
        <rdfs:comment xml:lang="en">Categories are &quot;surroundings&quot;, &quot;suppliers&quot;, &quot;skills&quot;, and  &quot;systems&quot;</rdfs:comment>
        <rdfs:label>Service industry 4S method</rdfs:label>
    </owl:NamedIndividual>
    


    <!-- https://w3id.org/ishikawa-diagram-ontology#5MandE -->


    <owl:NamedIndividual rdf:about="https://w3id.org/ishikawa-diagram-ontology#5MandE">
        <rdf:type rdf:resource="https://w3id.org/ishikawa-diagram-ontology#DesignPattern"/>
        <rdfs:comment xml:lang="en">The categories are &quot;measurement&quot;, &quot;materials&quot;, &quot;methods&quot;, &quot;manpower&quot;, and &quot;environment&quot;</rdfs:comment>
        <rdfs:label xml:lang="en">5M&amp;E structure</rdfs:label>
    </owl:NamedIndividual>
    


    <!-- https://w3id.org/ishikawa-diagram-ontology#8P -->


    <owl:NamedIndividual rdf:about="https://w3id.org/ishikawa-diagram-ontology#8P">
        <rdf:type rdf:resource="https://w3id.org/ishikawa-diagram-ontology#DesignPattern"/>
        <rdfs:comment xml:lang="en">The categories are &quot;price&quot;, &quot;people&quot;, &quot;place&quot;, &quot;procedure&quot;, &quot;promotion&quot;, &quot;processes&quot;, &quot;products&quot;, and &quot;policies&quot;</rdfs:comment>
        <rdfs:label xml:lang="en">Service industry 8P method</rdfs:label>
    </owl:NamedIndividual>
    


    <!-- https://www.kuleuven.be/kuleuven/ -->


    <owl:NamedIndividual rdf:about="https://www.kuleuven.be/kuleuven/">
        <rdfs:label>KU Leuven</rdfs:label>
        <foaf:name>KU Leuven</foaf:name>
    </owl:NamedIndividual>
</rdf:RDF>



<!-- Generated by the OWL API (version 5.1.18) https://github.com/owlcs/owlapi/ -->


